byteback-test/test-scala/src/main/scala/byteback/test/exceptions/Basic.scala
@@ -1,0 +1,61 @@
+/**
+ * RUN: %{byteback} -m -cp %{jar} -c %{class} -o %t.bpl
+ */
+package byteback.test.exceptions;
+
+import byteback.annotations.Contract._;
+import byteback.annotations.Special._;
+import byteback.annotations.Operator._;
+import byteback.annotations.Operator.{eq => equal};
+
+class Basic {
+
+  class ExceptionA extends Exception
+
+  class ExceptionB extends Exception
+
+  def tryCatchBlock(): Unit = {
+    try {
+      throw new Exception();
+    } catch {
+      case _: Exception =>
+    }
+  }
+
+  @Return
+  def neverThrows(): Unit = {
+
+  }
+
+  def neverCatches(): Unit = {
+    try {
+      neverThrows();
+    } catch {
+      case _: Exception => assertion(false);
+    }
+  }
+
+  @Predicate
+  def always_throws(e: Throwable): Boolean = {
+    return e.isInstanceOf[Exception];
+  }
+
+  @Ensure("always_throws")
+  def alwaysThrows(): Unit = {
+    throw new Exception();
+  }
+
+  def alwaysCatches(): Unit = {
+    try {
+      alwaysThrows();
+      assertion(false);
+    } catch {
+      case _: Throwable =>
+    }
+  }
+
+}
+/**
+ * RUN: %{verify} %t.bpl | filecheck %s
+ * CHECK: Boogie program verifier finished with 10 verified, 0 errors
+ */
